Checkpoint invariance w.r.t. validate

src/program_proof/tulip/res_replica.v
@@ -22,12 +22,12 @@ Section res.
       Persistent (is_replica_validated_ts γ gid rid ts).
     Admitted.
 
-    Lemma replica_validated_ts_insert γ gid rid vtss vts :
+    Lemma replica_validated_ts_insert {γ gid rid vtss} vts :
       own_replica_validated_tss γ gid rid vtss ==∗
       own_replica_validated_tss γ gid rid ({[vts]} ∪ vtss).
     Admitted.
 
-    Lemma replica_validated_ts_witness γ gid rid vtss vts :
+    Lemma replica_validated_ts_witness {γ gid rid vtss} vts :
       vts ∈ vtss ->
       own_replica_validated_tss γ gid rid vtss -∗
       is_replica_validated_ts γ gid rid vts.
@@ -127,6 +127,12 @@ Section res.
       lia.
     Qed.
 
+    Lemma replica_key_validation_big_update {γ gid rid kvdm} kvdm' :
+      map_Forall2 (λ _ l1 l2, prefix l1 l2) kvdm kvdm' ->
+      ([∗ map] k ↦ l ∈ kvdm, own_replica_key_validation γ gid rid k l) ==∗
+      ([∗ map] k ↦ l ∈ kvdm', own_replica_key_validation γ gid rid k l).
+    Admitted.
+
   End replica_key_validation.
 
   Section dura_hist.
@@ -173,6 +179,21 @@ Section res.
       ⌜ts2 = ts1⌝.
     Admitted.
 
+    Lemma replica_pts_big_agree {γ rid ptsm1 ptsm2} :
+      dom ptsm1 = dom ptsm2 ->
+      ([∗ map] k ↦ pts ∈ ptsm1, own_replica_pts_half γ rid k pts) -∗
+      ([∗ map] k ↦ pts ∈ ptsm2, own_replica_pts_half γ rid k pts) -∗
+      ⌜ptsm2 = ptsm1⌝.
+    Admitted.
+
+    Lemma replica_pts_big_update {γ rid ptsm} ptsm' :
+      dom ptsm = dom ptsm' ->
+      ([∗ map] k ↦ pts ∈ ptsm, own_replica_pts_half γ rid k pts) -∗
+      ([∗ map] k ↦ pts ∈ ptsm, own_replica_pts_half γ rid k pts) ==∗
+      ([∗ map] k ↦ pts ∈ ptsm', own_replica_pts_half γ rid k pts) ∗
+      ([∗ map] k ↦ pts ∈ ptsm', own_replica_pts_half γ rid k pts).
+    Admitted.
+
   End replica_pts.
 
   Section replica_spts.
@@ -195,7 +216,63 @@ Section res.
       ⌜ts2 = ts1⌝.
     Admitted.
 
+    Lemma replica_spts_big_agree {γ rid sptsm1 sptsm2} :
+      dom sptsm1 = dom sptsm2 ->
+      ([∗ map] k ↦ spts ∈ sptsm1, own_replica_spts_half γ rid k spts) -∗
+      ([∗ map] k ↦ spts ∈ sptsm2, own_replica_spts_half γ rid k spts) -∗
+      ⌜sptsm2 = sptsm1⌝.
+    Admitted.
+
+    Lemma replica_spts_big_update {γ rid sptsm} sptsm' :
+      dom sptsm = dom sptsm' ->
+      ([∗ map] k ↦ spts ∈ sptsm, own_replica_spts_half γ rid k spts) -∗
+      ([∗ map] k ↦ spts ∈ sptsm, own_replica_spts_half γ rid k spts) ==∗
+      ([∗ map] k ↦ spts ∈ sptsm', own_replica_spts_half γ rid k spts) ∗
+      ([∗ map] k ↦ spts ∈ sptsm', own_replica_spts_half γ rid k spts).
+    Admitted.
+
   End replica_spts.
+
+  Section replica_commit_map.
+
+    Definition own_replica_commit_map_half γ (rid : u64) (cm : gmap nat bool) : iProp Σ.
+    Admitted.
+
+    Lemma replica_commit_map_update {γ rid cm1 cm2} cm' :
+      own_replica_commit_map_half γ rid cm1 -∗
+      own_replica_commit_map_half γ rid cm2 ==∗
+      own_replica_commit_map_half γ rid cm' ∗
+      own_replica_commit_map_half γ rid cm'.
+    Admitted.
+
+    Lemma replica_commit_map_agree {γ rid cm1 cm2} :
+      own_replica_commit_map_half γ rid cm1 -∗
+      own_replica_commit_map_half γ rid cm2 -∗
+      ⌜cm2 = cm1⌝.
+    Admitted.
+
+  End replica_commit_map.
+
+  Section replica_currently_prepared_map.
+
+    Definition own_replica_currently_prepared_map_half
+      γ (rid : u64) (cpm : gmap nat dbmap) : iProp Σ.
+    Admitted.
+
+    Lemma replica_currently_prepared_map_update {γ rid cpm1 cpm2} cpm' :
+      own_replica_currently_prepared_map_half γ rid cpm1 -∗
+      own_replica_currently_prepared_map_half γ rid cpm2 ==∗
+      own_replica_currently_prepared_map_half γ rid cpm' ∗
+      own_replica_currently_prepared_map_half γ rid cpm'.
+    Admitted.
+
+    Lemma replica_currently_prepared_map_agree {γ rid cpm1 cpm2} :
+      own_replica_currently_prepared_map_half γ rid cpm1 -∗
+      own_replica_currently_prepared_map_half γ rid cpm2 -∗
+      ⌜cpm2 = cpm1⌝.
+    Admitted.
+
+  End replica_currently_prepared_map.
 
   Section replica_ballot.
 
