src/program_proof/tulip/invariance/validate.v
@@ -1,0 +1,179 @@
+From Perennial.program_proof.tulip Require Import prelude.
+
+Section validate.
+  Context `{!tulip_ghostG Σ}.
+
+  Lemma replica_inv_validate γ gid rid cpm psptsm ts pwrs :
+    (* cm !! ts = None -> *)
+    ts ≠ O ->
+    dom pwrs ⊆ keys_all ->
+    cpm !! ts = None ->
+    dom psptsm = dom pwrs ->
+    map_Forall (λ _ spts, (spts ≤ ts)%nat) psptsm ->
+    (* own_replica_commit_map_half γ rid cm -∗ *)
+    is_txn_pwrs γ gid ts pwrs -∗
+    own_replica_currently_prepared_map_half γ rid cpm -∗
+    ([∗ map] k ↦ spts ∈ psptsm, own_replica_spts_half γ rid k spts) -∗
+    ([∗ set] k ∈ dom pwrs, own_replica_pts_half γ rid k O) -∗
+    replica_inv γ gid rid ==∗
+    (* own_replica_commit_map_half γ rid cm ∗ *)
+    own_replica_currently_prepared_map_half γ rid (<[ts := pwrs]> cpm) ∗
+    ([∗ set] k ∈ dom pwrs, own_replica_spts_half γ rid k (S ts)) ∗
+    ([∗ set] k ∈ dom pwrs, own_replica_pts_half γ rid k ts) ∗
+    replica_inv γ gid rid ∗
+    is_replica_validated_ts γ gid rid ts.
+  Proof.
+    iIntros (Hnz Hdompwrs Hnp Hdompsptsm Hgespts) "#Hpwrs Hcpmprog Hpsptsmprog Hpptsmprog Hrp".
+    do 2 iNamed "Hrp".
+    (* Obtain facts about domain of the timestamp maps. *)
+    pose proof (map_Forall2_dom_L _ _ _ Hlenkvd) as Hdomsptsm.
+    symmetry in Hdomsptsm. rewrite Hdomkvdm in Hdomsptsm.
+    pose proof (map_Forall2_dom_L _ _ _ Hsptsmlk) as Hdomptsm.
+    symmetry in Hdomptsm. rewrite Hdomsptsm in Hdomptsm.
+    (* Take the relevant smallest preparable/prepare timestamps. *)
+    iDestruct (big_sepM_dom_subseteq_difference _ _ (dom pwrs) with "Hsptsm") as
+      (psptsm' [Hdompsptsm' Hsptsmincl]) "[Hpsptsm Hsptsm]".
+    { clear -Hdomsptsm Hdompwrs. set_solver. }
+    iDestruct (big_sepM_dom_subseteq_difference _ _ (dom pwrs) with "Hptsm") as
+      (pptsm [Hdompptsm Hptsmincl]) "[Hpptsm Hptsm]".
+    { clear -Hdomptsm Hdompwrs. set_solver. }
+    (* Agreements. *)
+    iDestruct (replica_currently_prepared_map_agree with "Hcpmprog Hcpm") as %->.
+    iDestruct (replica_spts_big_agree with "Hpsptsmprog Hpsptsm") as %->.
+    { by rewrite Hdompsptsm Hdompsptsm'. }
+    iDestruct (big_sepM_gset_to_gmap with "Hpptsmprog") as "Hpptsmprog".
+    iDestruct (replica_pts_big_agree with "Hpptsmprog Hpptsm") as %->.
+    { by rewrite dom_gset_to_gmap. }
+    (* Insert [(ts, pwrs)] into the currently-prepared txn map. *)
+    set cpm' := insert _ _ cpm.
+    iMod (replica_currently_prepared_map_update cpm' with "Hcpmprog Hcpm")
+      as "[Hcpmprog Hcpm]".
+    (* Set the smallest preparable timestamp to [S ts]. *)
+    set sptsm' := gset_to_gmap (S ts) (dom pwrs).
+    iMod (replica_spts_big_update sptsm' with "Hpsptsmprog Hpsptsm")
+      as "[Hpsptsmprog Hpsptsm]".
+    { by rewrite dom_gset_to_gmap Hdompsptsm. }
+    (* Set the prepare timestamp to [ts]. *)
+    set ptsm' := gset_to_gmap ts (dom pwrs).
+    iMod (replica_pts_big_update ptsm' with "Hpptsmprog Hpptsm") as "[Hpptsmprog Hpptsm]".
+    { by rewrite 2!dom_gset_to_gmap. }
+    rewrite 2!big_sepM_gset_to_gmap.
+    (* Insert [ts] into the set of validated timestamps [vtss]. *)
+    iMod (replica_validated_ts_insert ts with "Hvtss") as "Hvtss".
+    iDestruct (replica_validated_ts_witness ts with "Hvtss") as "#Htsvd".
+    { set_solver. }
+    iFrame "Hcpm Hpsptsmprog Hpptsmprog Htsvd".
+    (* Put the relevant smallest preparable/prepare timestamps back. *)
+    iDestruct (big_sepM_gset_to_gmap with "Hpsptsm") as "Hpsptsm".
+    iCombine "Hpsptsm Hsptsm" as "Hsptsm".
+    rewrite -big_sepM_union; last first.
+    { rewrite map_disjoint_dom dom_gset_to_gmap.
+      clear -Hdomsptsm Hdompsptsm. set_solver.
+    }
+    rewrite map_union_difference_union_L; last first.
+    { by rewrite dom_gset_to_gmap Hdompsptsm. }
+    iDestruct (big_sepM_gset_to_gmap with "Hpptsm") as "Hpptsm".
+    iCombine "Hpptsm Hptsm" as "Hptsm".
+    rewrite -big_sepM_union; last first.
+    { rewrite map_disjoint_dom dom_gset_to_gmap.
+      clear -Hdomptsm Hdompptsm. set_solver.
+    }
+    rewrite map_union_difference_union_L; last first.
+    { by rewrite dom_gset_to_gmap Hdompptsm. }
+    (* Extend the validation list for each [k ∈ dom pwrs]. *)
+    set extendf := λ (ov : option dbval) (ol : option (list bool)),
+                     match ov, ol with
+                     | Some _, Some l => Some (extend ts false l ++ [true])
+                     | None, Some l => Some l
+                     | _, _ => None
+                     end.
+    set kvdm' := merge extendf pwrs kvdm.
+    unshelve epose proof (gmap_nonexpanding_merge_dom pwrs kvdm extendf _)
+      as Hdomkvdm'.
+    { intros ov ol. by destruct ov, ol. }
+    iMod (replica_key_validation_big_update kvdm' with "Hkvdm") as "Hkvdm".
+    { rewrite map_Forall2_forall.
+      split; last first.
+      { symmetry. apply Hdomkvdm'. }
+      intros k l l' Hl Hl'.
+      destruct (pwrs !! k) as [v |] eqn:Hpwrsk;
+        rewrite lookup_merge Hl Hpwrsk /= in Hl'; inv Hl'; last done.
+      apply prefix_app_r, extend_prefix.
+    }
+    (* Obtain witnesses that key [k ∈ dom pwrs] has been validated. *)
+    iAssert (validated_pwrs_of_txn γ gid rid ts)%I as "#Hvkeys".
+    { iFrame "Hpwrs".
+      iDestruct (big_sepM_dom_subseteq_difference _ _ (dom pwrs) with "Hkvdm")
+        as (m [Hdomm Hincl]) "[Hkvdm _]".
+      { rewrite Hdomkvdm' Hdomkvdm. apply Hdompwrs. }
+      iApply (big_sepM_sepS_impl with "Hkvdm"); first apply Hdomm.
+      iIntros (k l Hl) "!> Hkvd".
+      iDestruct (replica_key_validation_witness with "Hkvd") as "#Hlb".
+      iFrame "Hlb".
+      iPureIntro.
+      pose proof (lookup_weaken _ _ _ _ Hl Hincl) as Hl'.
+      apply elem_of_dom_2 in Hl.
+      assert (is_Some (pwrs !! k)) as [v Hv].
+      { by rewrite -elem_of_dom -Hdomm. }
+      assert (is_Some (kvdm !! k)) as [vl Hvl].
+      { rewrite -elem_of_dom Hdomkvdm. clear -Hl Hdomm Hdompwrs. set_solver. }
+      rewrite lookup_merge Hv Hvl /= in Hl'.
+      inv Hl'.
+      assert (is_Some (psptsm !! k)) as [spts Hspts].
+      { by rewrite -elem_of_dom Hdompsptsm -Hdomm. }
+      specialize (Hgespts _ _ Hspts). simpl in Hgespts.
+      pose proof (lookup_weaken _ _ _ _ Hspts Hsptsmincl) as Hspts'.
+      pose proof (map_Forall2_lookup_Some _ _ _ _ _ _ Hvl Hspts' Hlenkvd) as Hlenvl.
+      simpl in Hlenvl.
+      rewrite lookup_snoc_Some.
+      right.
+      split; last done.
+      rewrite extend_length.
+      clear -Hlenvl Hgespts. lia.
+    }
+    iFrame "∗ # %".
+    iModIntro.
+    iSplit.
+    { by iApply big_sepM_insert_2. }
+    iSplit.
+    { by iApply big_sepS_insert_2. }
+    iSplit.
+    { iIntros (k t).
+      admit.
+    }
+    iPureIntro.
+    split.
+    { rewrite dom_insert_L. clear -Hvtss. set_solver. }
+    split.
+    { by rewrite Hdomkvdm'. }
+    split.
+    { admit. }
+    split.
+    { admit. }
+    split.
+    { intros t w k Hw Hk.
+      destruct (decide (t = ts)) as [-> | Hne]; last first.
+      { rewrite lookup_insert_ne in Hw; last done.
+        specialize (Hpil _ _ _ Hw Hk).
+        destruct (decide (k ∈ dom pwrs)) as [Hin | Hnotin].
+        { exfalso.
+          assert (Hz : ptsm !! k = Some O).
+          { unshelve eapply (lookup_weaken _ _ _ _ _ Hptsmincl).
+            by rewrite lookup_gset_to_gmap_Some.
+          }
+          clear -Hz Hpil Hw Hcpmnz.
+          inv Hz.
+        }
+        rewrite lookup_union_r; last first.
+        { by rewrite lookup_gset_to_gmap_None. }
+        apply Hpil.
+      }
+      rewrite lookup_insert in Hw.
+      symmetry in Hw. inv Hw.
+      apply lookup_union_Some_l.
+      by rewrite lookup_gset_to_gmap_Some.
+    }
+    { by rewrite lookup_insert_ne. }
+  Admitted.
+
+End validate.
